experiment/Experiment.Repr.Fun.fst
@@ -1,0 +1,81 @@
+module Experiment.Repr.Fun
+
+noeq
+type prog_tree : (a : Type) -> Type =
+  | Tnew   : (a : Type) -> prog_tree a
+  | Tasrt  : (p : prop) -> prog_tree unit
+  | Tasum  : (p : prop) -> prog_tree unit
+  | Tret   : (a : Type) -> (x : a) -> prog_tree a
+  | Tbind  : (a : Type) -> (b : Type) ->
+             (f : prog_tree a) -> (g : a -> prog_tree b) ->
+             prog_tree b
+  | TbindP : (a : Type) -> (b : Type) ->
+             (wp : pure_wp a) -> (x : unit -> PURE a wp) -> (g : a -> prog_tree b) ->
+             prog_tree b
+
+let return (#a : Type) (x : a) : prog_tree a
+  = Tret a x
+
+let bind (#a #b : Type) (f : prog_tree a) (g : a -> prog_tree b) : prog_tree b
+  = Tbind a b f g
+
+
+let rec tree_req (#a : Type) (t : prog_tree a)
+  : Tot pure_pre (decreases t)
+  = match t with
+  | Tnew   _          -> True
+  | Tasrt  p          -> p
+  | Tasum  _          -> True
+  | Tret   _ _        -> True
+  | Tbind  a _ f g    -> tree_req f /\ (forall (x : a) . tree_ens f x ==> tree_req (g x))
+  | TbindP a _ wp _ g -> wp (fun x -> tree_req (g x)) /\ True
+
+and tree_ens (#a : Type) (t : prog_tree a)
+  : Tot (pure_post a) (decreases t)
+  = match t with
+  | Tnew   _          -> fun _  -> True
+  | Tasrt  p          -> fun () -> True (* p ?*)
+  | Tasum  p          -> fun () -> p
+  | Tret   _ x        -> fun r  -> r == x
+  | Tbind  a _ f g    -> fun y  -> exists (x : a) . tree_ens f x /\ tree_ens (g x) y
+  | TbindP a _ wp _ g -> fun y -> as_requires wp /\ (exists (x : a) . as_ensures wp x /\ tree_ens (g x) y)
+
+
+module MP = FStar.Monotonic.Pure
+module T  = FStar.Tactics
+module U  = Learn.Util
+open FStar.Classical.Sugar
+
+
+let rec tree_wp (#a : Type) (t : prog_tree a)
+  : Tot (pure_wp a) (decreases t)
+  = match t with
+  | Tnew  a           -> MP.as_pure_wp (fun pt -> forall (x : a) . pt x)
+  | Tasrt p           -> MP.as_pure_wp (fun pt -> p /\ (p ==> pt ()))
+  | Tasum p           -> MP.as_pure_wp (fun pt -> p ==> pt ())
+  | Tret  _ x         -> MP.as_pure_wp (fun pt -> pt x)
+  | Tbind a _ f g     -> MP.elim_pure_wp_monotonicity_forall ();
+                        MP.as_pure_wp (fun pt -> tree_wp f (fun (x : a) -> tree_wp (g x) pt))
+  | TbindP a _ wp _ g -> MP.elim_pure_wp_monotonicity_forall ();
+                        MP.as_pure_wp (fun pt -> wp (fun (x : a) -> tree_wp (g x) pt))
+
+let rec tree_wp_sound (#a : Type) (t : prog_tree a) (post : pure_post a)
+  : Lemma (requires tree_wp t post)
+          (ensures  tree_req t /\ (forall (x : a) . tree_ens t x ==> post x))
+  = match t with
+  | Tnew _ | Tasrt _ | Tasum _ | Tret _ _ -> ()
+  | Tbind a b f g ->
+      let post1 (x : a) = tree_wp (g x) post in
+      assert (tree_wp (Tbind a b f g) post == tree_wp f post1) by T.(trefl ());
+      tree_wp_sound f post1;
+      introduce forall (x : a) . tree_wp (g x) post ==> (tree_req (g x) /\ (forall (y : b) . tree_ens (g x) y ==> post y))
+        with introduce _ ==> _ with _ . tree_wp_sound (g x) post
+  | TbindP a b wp xf g ->
+      let post1 (x : a) = tree_wp (g x) post in
+      let req1  (x : a) = tree_req (g x)     in
+      assert (tree_wp (TbindP a b wp xf g) post == wp post1) by T.(trefl ());
+      MP.elim_pure_wp_monotonicity wp;
+      introduce forall (x : a) . post1 x ==> (req1 x /\ (forall (y : b) . tree_ens (g x) y ==> post y))
+        with introduce _ ==> _ with _ . tree_wp_sound (g x) post;
+      assert (tree_req (TbindP a b wp xf g) == (wp req1 /\ True)) by T.(trefl ());
+      U.prop_equal (fun p -> p) (wp req1 /\ True) (tree_req (TbindP a b wp xf g))
