experiment/Experiment.Steel.Repr.ST.fst
@@ -1,0 +1,412 @@
+module Experiment.Steel.Repr.ST
+
+module U    = Learn.Util
+module M    = Experiment.Steel.Repr.M
+module L    = FStar.List.Pure
+module Uv   = FStar.Universe
+module Perm = Learn.Permutation
+
+open Experiment.Steel.Repr.M
+open Steel.Effect.Common
+
+
+(* TODO? define vequiv for [list a] *)
+let vequiv (ts0 ts1 : ty_list) = f : Perm.perm_f (L.length ts0) {ts1 == Perm.apply_perm_r f ts0}
+
+unfold
+let apply_vequiv (#ts0 #ts1 : ty_list) (f : vequiv ts0 ts1) (xs : var_list ts0) : var_list ts1
+  = var_apply_perm_r f xs
+
+unfold
+let var_split_at_ty (ts0 ts1 : ty_list) (xs : var_list L.(ts0@ts1))
+  : var_list ts0 & var_list ts1
+  = L.lemma_append_splitAt ts0 ts1;
+    var_splitAt (L.length ts0) xs
+
+
+type pre_t = ty_list
+type post_t (a : Type) = a -> ty_list
+type req_t (pre : pre_t) = var_list pre -> prop
+type ens_t (pre : pre_t) (a : Type) (post : post_t a) = var_list pre -> (x : a) -> var_list (post x) -> prop
+
+
+type unit' : Type u#a = | Unit' : unit'
+
+noeq
+type prog_tree : (a : Type u#a) -> (pre : pre_t u#b) -> (post : post_t u#a u#b a) -> Type u#(1 + max a b) =
+  | Tequiv : (pre : ty_list) -> (post : ty_list) ->
+             (p : vequiv pre post) ->
+             prog_tree unit' pre (fun _ -> post)
+  | Tspec  : (a : Type u#a) -> (pre : pre_t) -> (post : post_t a) -> (frame : ty_list) ->
+             (req : req_t pre) -> (ens : ens_t pre a post) ->
+             prog_tree a L.(pre@frame) (fun (x : a) -> L.(post x @ frame))
+  | Tret   : (a : Type u#a) -> (x : a) -> (post : post_t a) ->
+             prog_tree a (post x) post
+  | Tbind  : (a : Type u#a) -> (b : Type u#a) ->
+             (pre : pre_t) -> (itm : (a -> ty_list)) -> (post : post_t b) ->
+             (f : prog_tree a pre itm) -> (g : ((x : a) -> prog_tree b (itm x) post)) ->
+             prog_tree b pre post
+  | TbindP : (a : Type u#a) -> (b : Type u#a) ->
+             (pre : pre_t) -> (post : post_t b) ->
+             (wp : pure_wp a) -> (x : unit -> PURE a wp) -> (g : a -> prog_tree b pre post) ->
+             prog_tree b pre post
+
+let bind (#a : Type) (#b : Type) (#pre : pre_t) (#itm : a -> ty_list) (#post : post_t b)
+         (f : prog_tree a pre itm) (g : (x:a) -> prog_tree b (itm x) post)
+  : prog_tree b pre post
+  = Tbind a b pre itm post f g
+
+(* TODO? generalize Experiment.Steel.Repr.M.bind_req... *)
+let rec tree_req (#a : Type) (#pre : pre_t) (#post : post_t a) (t : prog_tree a pre post)
+  : Tot (req_t pre) (decreases t)
+  = match t with
+  | Tequiv _ _ _ ->
+             (fun sl0 -> True)
+  | Tspec _  pre _ frame  req _ ->
+             (fun sl0 -> req (var_split_at_ty pre frame sl0)._1)
+  | Tret _ _ _ ->
+             (fun sl0 -> True)
+  | Tbind a _  _ itm _  f g ->
+             (fun sl0 -> tree_req f sl0 /\
+               (forall (x : a) (sl1 : var_list (itm x)) . tree_ens f sl0 x sl1 ==> tree_req (g x) sl1))
+  | TbindP a _  _ _  wp _ g ->
+             (fun sl0 -> wp (fun (x : a) -> tree_req (g x) sl0) /\ True)
+
+and tree_ens (#a : Type) (#pre : pre_t) (#post : post_t a) (t : prog_tree a pre post)
+  : Tot (ens_t pre a post) (decreases t)
+  = match t with
+  | Tequiv _ _ p ->
+             (fun sl0 _ sl1 -> sl1 == apply_vequiv p sl0)
+  | Tspec _  pre post frame  req ens ->
+             (fun sl0 x sl1 ->
+               let sl0', frame0 = var_split_at_ty pre      frame sl0 in
+               let sl1', frame1 = var_split_at_ty (post x) frame sl1 in
+               frame1 == frame0 /\ ens sl0' x sl1')
+  | Tret _ x post ->
+             (fun sl0 x' sl1 -> x' == x /\ sl1 == sl0)
+  | Tbind a _  _ itm _  f g ->
+             (fun sl0 y sl2 -> tree_req f sl0 /\
+               (exists (x : a) (sl1 : var_list (itm x)) . tree_ens f sl0 x sl1 /\ tree_ens (g x) sl1 y sl2))
+  | TbindP a _  _ _  wp _ g ->
+             (fun sl0 y sl1 -> as_requires wp /\ (exists (x : a) . as_ensures wp x /\ tree_ens (g x) sl0 y sl1))
+
+
+(*** Repr.M --> Repr.ST *)
+
+module T = FStar.Tactics
+open FStar.Calc
+
+unfold
+let vequiv_of_M (#src #dst : vprop_list) (p : M.vequiv src dst)
+  : Pure (vequiv (vprop_list_sels_t src) (vprop_list_sels_t dst))
+         (requires True) (ensures fun p' ->
+           U.cast #(Perm.perm_f (L.length (vprop_list_sels_t src))) (Perm.perm_f (L.length src)) p' == p)
+  = Perm.map_apply_r p Mkvprop'?.t src;
+    U.cast #(Perm.perm_f (L.length src)) (Perm.perm_f (L.length (vprop_list_sels_t src))) p
+
+let rec repr_ST_of_M (#a : Type u#a) (t : M.prog_tree a)
+                     (#pre : M.pre_t) (#post : M.post_t a) (c : M.tree_cond t pre post)
+  : Tot (prog_tree a (vprop_list_sels_t pre) (fun (x : a) -> vprop_list_sels_t (post x)))
+        (decreases t)
+  = match c with
+  | TCspec #a #pre #post #req #ens  pre' post' frame  p0 p1 ->
+             Tequiv (vprop_list_sels_t pre') (vprop_list_sels_t L.(pre@frame)) (vequiv_of_M p0);;
+             (**) L.map_append Mkvprop'?.t pre frame;
+             x <-- Tspec a (vprop_list_sels_t pre) (fun (x : a) -> vprop_list_sels_t (post x))
+                          (vprop_list_sels_t frame) req ens;
+             (**) L.map_append Mkvprop'?.t (post x) frame;
+             Tequiv (vprop_list_sels_t L.(post x@frame)) (vprop_list_sels_t (post' x)) (vequiv_of_M (p1 x));;
+             Tret _ x (fun x -> vprop_list_sels_t (post' x))
+  | TCret #a #x  pre post  p ->
+             Tequiv (vprop_list_sels_t pre) (vprop_list_sels_t (post x)) (vequiv_of_M p);;
+             Tret _ x (fun x -> vprop_list_sels_t (post x))
+  | TCbind #a #b #f #g  pre itm post  cf cg ->
+             x <-- repr_ST_of_M f cf;
+             repr_ST_of_M (g x) (cg x)
+  | TCbindP #a #b #wp #x #g  pre post  cg ->
+             TbindP a b _ _ wp x (fun x -> repr_ST_of_M (g x) (cg x))
+
+
+let norm_tree_spec () : T.Tac unit
+  = T.norm [delta_only [`%repr_ST_of_M; `%bind; `%tree_req; `%tree_ens];
+            zeta; iota; simplify]
+
+unfold
+let vequiv_sym (#ts0 #ts1 : ty_list) (f : vequiv ts0 ts1) : vequiv ts1 ts0
+  = 
+    Perm.(calc (==) {
+      apply_perm_r (inv_f f) ts1;
+    == {}
+      apply_perm_r (inv_f f) (apply_perm_r f ts0);
+    == {apply_r_comp (inv_f f) f ts0}
+      ts0;
+    });
+    U.cast #(Perm.perm_f (L.length ts0)) (Perm.perm_f (L.length ts1)) (Perm.inv_f f)
+
+let vequiv_ts_eq (#ts0 #ts1 : ty_list) (f : vequiv ts0 ts1)
+  : Lemma (ts1 == Perm.apply_perm_r f ts0)
+  = ()
+
+let apply_vequiv_sym_l (#ts0 #ts1 : ty_list) (f : vequiv ts0 ts1) (xs : var_list ts0)
+  : Lemma (apply_vequiv (vequiv_sym f) (apply_vequiv f xs) == xs)
+  =
+    var_apply_r_comp (Perm.inv_f f) f xs
+
+let apply_vequiv_sym_r (#ts0 #ts1 : ty_list) (f : vequiv ts0 ts1) (xs : var_list ts1)
+  : Lemma (apply_vequiv f (apply_vequiv (vequiv_sym f) xs) == xs)
+  =
+    vequiv_ts_eq (vequiv_sym f);
+    var_apply_r_comp f (Perm.inv_f f) xs
+
+
+let apply_vequiv_sym_eq_iff (#ts0 #ts1 : ty_list) (f : vequiv ts0 ts1) (xs : var_list ts0) (ys : var_list ts1)
+  : Lemma (xs == apply_vequiv (vequiv_sym f) ys <==> ys == apply_vequiv f xs)
+  =
+    apply_vequiv_sym_l f xs;
+    apply_vequiv_sym_r f ys
+
+#push-options "--z3rlimit 15"
+let repr_ST_of_M__TCspec_ens
+      #a #pre #post (req : M.req_t pre) (ens : M.ens_t pre a post)
+      (pre' : M.pre_t) (post' : M.post_t a) (frame : vprop_list)
+      (p0 : M.vequiv pre' L.(pre @ frame)) (p1 : (x : a) -> M.vequiv (post x @ frame) (post' x))
+      (sl0' : sl_t pre') (res : a) (sl1' : sl_t (post' res))
+
+  : Lemma (
+    (**) L.map_append Mkvprop'?.t pre frame;
+    (**) L.map_append Mkvprop'?.t (post res) frame;
+
+    (tree_ens (repr_ST_of_M _ (TCspec #a #pre #post #req #ens  pre' post' frame  p0 p1)) sl0' res sl1'
+    <==> (let sl0, frame0 = var_split_at_ty (vprop_list_sels_t pre) (vprop_list_sels_t frame)
+                             (apply_vequiv (vequiv_of_M p0) sl0') in
+        let sl1, frame1 = var_split_at_ty (vprop_list_sels_t (post res)) (vprop_list_sels_t frame)
+                             (apply_vequiv (vequiv_sym (vequiv_of_M (p1 res))) sl1') in
+        req sl0 /\ frame1 == frame0 /\ ens sl0 res sl1)))
+  =
+    L.map_append Mkvprop'?.t pre frame;
+    L.map_append Mkvprop'?.t (post res) frame;
+    assert (
+      tree_ens (repr_ST_of_M _ (TCspec #a #pre #post #req #ens  pre' post' frame  p0 p1)) sl0' res sl1'
+    <==> (exists (sl1f : var_list L.(vprop_list_sels_t (post res) @ vprop_list_sels_t frame)) .
+          let sl0, frame0 = var_split_at_ty (vprop_list_sels_t pre) (vprop_list_sels_t frame)
+                               (apply_vequiv (vequiv_of_M p0) sl0') in
+          let sl1, frame1 = var_split_at_ty (vprop_list_sels_t (post res)) (vprop_list_sels_t frame) sl1f in
+          sl1' == apply_vequiv (vequiv_of_M (p1 res)) sl1f /\
+          req sl0 /\ frame1 == frame0 /\ ens sl0 res sl1))
+      by T.(norm_tree_spec (); smt ());
+    
+    introduce forall (sl1f : var_list L.(vprop_list_sels_t (post res) @ vprop_list_sels_t frame)) .
+        sl1' == apply_vequiv (vequiv_of_M (p1 res)) sl1f <==>
+        sl1f == apply_vequiv (vequiv_sym (vequiv_of_M (p1 res))) sl1'
+      with apply_vequiv_sym_eq_iff (vequiv_of_M (p1 res)) sl1f sl1';
+
+    assert (tree_ens (repr_ST_of_M _ (TCspec #a #pre #post #req #ens  pre' post' frame  p0 p1)) sl0' res sl1'
+    <==> (let sl0, frame0 = var_split_at_ty (vprop_list_sels_t pre) (vprop_list_sels_t frame)
+                             (apply_vequiv (vequiv_of_M p0) sl0') in
+        let sl1, frame1 = var_split_at_ty (vprop_list_sels_t (post res)) (vprop_list_sels_t frame)
+                             (apply_vequiv (vequiv_sym (vequiv_of_M (p1 res))) sl1') in
+        req sl0 /\ frame1 == frame0 /\ ens sl0 res sl1))
+#pop-options
+
+
+/// Remark: the equivalence of the ensures clauses holds only when the requires clause is satisfied
+
+#push-options "--z3rlimit 30"
+let rec repr_ST_of_M_req (#a : Type) (t : M.prog_tree a)
+                         (#pre : M.pre_t) (#post : M.post_t a) (c : M.tree_cond t pre post)
+                         (sl0 : sl_t pre)
+  : Lemma (ensures M.tree_req t c sl0 <==> tree_req (repr_ST_of_M t c) sl0)
+  = match c as c returns squash (M.tree_req t c sl0 <==> tree_req (repr_ST_of_M t c) sl0) with
+  | TCspec #a #pre #post #req #ens  pre' post' frame  p0 p1 ->
+             L.map_append Mkvprop'?.t pre frame;
+
+             calc (<==>) {
+               M.tree_req _ (TCspec #a #pre #post #req #ens  pre' post' frame  p0 p1) sl0;
+             <==> {_ by T.(apply_lemma (`U.iff_refl); trefl ()) }
+               req (extract_vars_f pre' pre frame p0 sl0)._1;
+             <==> { assert_norm (extract_vars_f pre' pre frame p0 sl0
+                    == var_split_at_ty (vprop_list_sels_t pre) (vprop_list_sels_t frame)
+                         (apply_vequiv (vequiv_of_M p0) sl0)) }
+               req (var_split_at_ty (vprop_list_sels_t pre) (vprop_list_sels_t frame)
+                              (apply_vequiv (vequiv_of_M p0) sl0))._1;
+             <==> { assert (tree_req (repr_ST_of_M _ (TCspec #a #pre #post #req #ens  pre' post' frame  p0 p1)) sl0
+                     <==> req (var_split_at_ty (vprop_list_sels_t pre) (vprop_list_sels_t frame)
+                              (apply_vequiv (vequiv_of_M p0) sl0))._1)
+                 by T.(norm_tree_spec (); smt ()) }
+               tree_req (repr_ST_of_M _ (TCspec #a #pre #post #req #ens  pre' post' frame  p0 p1)) sl0;
+             <==> { U.f_equal tree_req (repr_ST_of_M _ (TCspec #a #pre #post #req #ens  pre' post' frame  p0 p1))
+                                     (repr_ST_of_M _ c) }
+               tree_req (repr_ST_of_M _ c) sl0;
+             }
+
+  | TCret #a #x  pre post  p ->
+             U.f_equal tree_req (repr_ST_of_M _ (TCret #a #x pre post p))
+                                (repr_ST_of_M _ c);
+             assert (M.tree_req _ (TCret #a #x pre post p) sl0 == True) by T.(trefl ());
+             assert (tree_req (repr_ST_of_M _ (TCret #a #x pre post p)) sl0 <==> True)
+                    by T.(norm_tree_spec (); smt ())
+
+  | TCbind #a #b #f #g  pre itm post  cf cg ->
+             let r0 = repr_ST_of_M _ (TCbind #a #b #f #g  pre itm post  cf cg) in
+             let r1 = repr_ST_of_M _ c in
+             U.f_equal tree_req r0 r1;
+
+             calc (<==>) {
+               M.tree_req _ (TCbind #a #b #f #g  pre itm post  cf cg) sl0;
+             <==> {_ by T.(apply_lemma (`U.iff_refl); trefl ())}
+               bind_req (M.tree_req f cf) (M.tree_ens f cf) (fun x -> M.tree_req (g x) (cg x)) sl0;
+             <==> {
+               repr_ST_of_M_req f cf sl0;
+               introduce forall (x : a) (sl1 : sl_t (itm x)) .
+                 tree_req (repr_ST_of_M f cf) sl0 ==>
+                 (M.tree_ens f cf sl0 x sl1 <==> tree_ens (repr_ST_of_M f cf) sl0 x sl1) /\
+                 (M.tree_req (g x) (cg x) sl1 <==> tree_req (repr_ST_of_M (g x) (cg x)) sl1)
+               with introduce _ ==> _
+               with _ . (repr_ST_of_M_ens f cf sl0 x sl1; repr_ST_of_M_req (g x) (cg x) sl1)
+             }
+               tree_req (repr_ST_of_M f cf) sl0 /\
+               (forall (x : a) (sl1 : var_list (vprop_list_sels_t (itm x))) .
+                 tree_ens (repr_ST_of_M f cf) sl0 x sl1 ==> tree_req (repr_ST_of_M (g x) (cg x)) sl1);
+             <==> {_ by T.(apply_lemma (`U.iff_refl); trefl ())}
+               tree_req (repr_ST_of_M _ (TCbind #a #b #f #g  pre itm post  cf cg)) sl0;
+             <==> {}
+               tree_req r0 sl0;
+             <==> { assert (r0 == r1) }
+               tree_req r1 sl0;
+             }
+
+  | TCbindP #a #b #wp #x #g  pre post  cg ->
+            calc (<==>) {
+              M.tree_req _ c sl0;
+            <==> {}
+              M.tree_req _ (TCbindP #a #b #wp #x #g pre post cg) sl0;
+            <==> {_ by T.(apply_lemma (`U.iff_refl); trefl ())}
+              bind_pure_req wp (fun x -> M.tree_req (g x) (cg x)) sl0;
+            <==> {
+              FStar.Monotonic.Pure.elim_pure_wp_monotonicity wp;
+              introduce forall (x : a).
+                 (M.tree_req (g x) (cg x) sl0 <==> tree_req (repr_ST_of_M (g x) (cg x)) sl0)
+               with repr_ST_of_M_req (g x) (cg x) sl0
+            }
+              wp (fun x -> tree_req (repr_ST_of_M (g x) (cg x)) sl0) /\ True;
+            <==> {_ by T.(apply_lemma (`U.iff_refl); trefl ())}
+              tree_req (repr_ST_of_M _ (TCbindP #a #b #wp #x #g pre post cg)) sl0;
+            <==> {U.f_equal tree_req (repr_ST_of_M _ (TCbindP #a #b #wp #x #g pre post cg)) (repr_ST_of_M _ c)}
+              tree_req (repr_ST_of_M _ c) sl0;
+            }
+
+and repr_ST_of_M_ens (#a : Type) (t : M.prog_tree a)
+                     (#pre : M.pre_t) (#post : M.post_t a) (c : M.tree_cond t pre post)
+                     (sl0 : sl_t pre) (res : a) (sl1 : sl_t (post res))
+  : Lemma (requires M.tree_req t c sl0)
+          (ensures M.tree_ens t c sl0 res sl1 <==> tree_ens (repr_ST_of_M t c) sl0 res sl1)
+  = match c as c returns squash (M.tree_ens t c sl0 res sl1 <==> tree_ens (repr_ST_of_M t c) sl0 res sl1) with
+    | TCspec #a #pre #post #req #ens  pre' post' frame  p0 p1 ->
+             L.map_append Mkvprop'?.t pre frame;
+             L.map_append Mkvprop'?.t (post res) frame;
+
+             calc (<==>) {
+               M.tree_ens _ (TCspec #a #pre #post #req #ens  pre' post' frame  p0 p1) sl0 res sl1;
+             <==> {_ by T.(apply_lemma (`U.iff_refl); trefl ()) }
+              (let fsl0, frame0 = extract_vars_f pre' pre frame p0 sl0 in
+               let fsl1, frame1 = extract_vars_f (post' res) (post res) frame (M.vequiv_sym (p1 res)) sl1 in
+                frame1 == frame0 /\ ens fsl0 res fsl1);
+             <==> { (* since req holds *) }
+              (let fsl0, frame0 = var_split_at_ty (vprop_list_sels_t pre) (vprop_list_sels_t frame)
+                                                  (apply_vequiv (vequiv_of_M p0) sl0) in
+               let fsl1, frame1 = var_split_at_ty (vprop_list_sels_t (post res)) (vprop_list_sels_t frame)
+                                                  (apply_vequiv (vequiv_sym (vequiv_of_M (p1 res))) sl1) in
+                req fsl0 /\ frame1 == frame0 /\ ens fsl0 res fsl1);
+             <==> {repr_ST_of_M__TCspec_ens req ens pre' post' frame p0 p1 sl0 res sl1}
+               tree_ens (repr_ST_of_M _ (TCspec #a #pre #post #req #ens  pre' post' frame p0 p1)) sl0 res sl1;
+             <==> {U.f_equal tree_ens (repr_ST_of_M _ (TCspec #a #pre #post #req #ens  pre' post' frame  p0 p1))
+                                    (repr_ST_of_M _ c)}
+               tree_ens (repr_ST_of_M _ c) sl0 res sl1;
+             }
+
+  | TCret #a #x  pre post  p ->
+             calc (<==>) {
+               M.tree_ens _ (TCret #a #x pre post p) sl0 res sl1;
+             <==> { assert (M.tree_ens _ (TCret #a #x pre post p) sl0 res sl1 <==>
+                           (res == x /\ sl1 == extract_vars p sl0))
+                      by T.(norm [delta_only [`%M.tree_ens]; zeta; iota]; smt ()) }
+               res == x /\ sl1 == extract_vars p sl0;
+             <==> {}
+               res == x /\ sl1 == apply_vequiv (vequiv_of_M p) sl0;
+             <==> { assert (tree_ens (repr_ST_of_M _ (TCret #a #x pre post p)) sl0 res sl1 <==>
+                           (res == x /\ sl1 == apply_vequiv (vequiv_of_M p) sl0))
+                      by T.(norm_tree_spec (); smt ()) }
+               tree_ens (repr_ST_of_M _ (TCret #a #x pre post p)) sl0 res sl1;
+             <==> { U.f_equal tree_ens (repr_ST_of_M _ (TCret #a #x pre post p))
+                                    (repr_ST_of_M _ c) }
+               tree_ens (repr_ST_of_M _ c) sl0 res sl1;
+             }
+
+  | TCbind #a #b #f #g  pre itm post  cf cg ->
+             calc (<==>) {
+               M.tree_ens _ (TCbind #a #b #f #g  pre itm post  cf cg) sl0 res sl1;
+             <==> {_ by T.(apply_lemma (`U.iff_refl); trefl ())}
+               bind_ens (M.tree_req f cf) (M.tree_ens f cf) (fun x -> M.tree_ens (g x) (cg x)) sl0 res sl1;
+             <==> {
+               repr_ST_of_M_req f cf sl0;
+               introduce forall (x : a) (sl1' : sl_t (itm x)) .
+                 tree_req (repr_ST_of_M f cf) sl0 ==>
+                 (M.tree_ens f cf sl0 x sl1' <==> tree_ens (repr_ST_of_M f cf) sl0 x sl1') /\
+                 (M.tree_ens f cf sl0 x sl1' ==> (
+                 (M.tree_ens (g x) (cg x) sl1' res sl1 <==> tree_ens (repr_ST_of_M (g x) (cg x)) sl1' res sl1)))
+               with introduce _ ==> _ with _ . introduce _ /\ _
+               with repr_ST_of_M_ens f cf sl0 x sl1'
+                and introduce _ ==> _
+                with _ . repr_ST_of_M_ens (g x) (cg x) sl1' res sl1
+             }
+               tree_req (repr_ST_of_M f cf) sl0 /\
+               (exists (x : a) (sl1' : var_list (vprop_list_sels_t (itm x))) .
+                 tree_ens (repr_ST_of_M f cf) sl0 x sl1' /\
+                 tree_ens (repr_ST_of_M (g x) (cg x)) sl1' res sl1);
+             <==> {_ by T.(apply_lemma (`U.iff_refl); trefl ())}
+               tree_ens (repr_ST_of_M _ (TCbind #a #b #f #g  pre itm post  cf cg)) sl0 res sl1;
+             <==> {U.f_equal tree_ens (repr_ST_of_M _ (TCbind #a #b #f #g pre itm post cf cg))
+                                    (repr_ST_of_M _ c)}
+               tree_ens (repr_ST_of_M _ c) sl0 res sl1;
+             }
+
+  | TCbindP #a #b #wp #x #g  pre post  cg ->
+            calc (<==>) {
+              M.tree_ens _ c sl0 res sl1;
+            <==> {}
+              M.tree_ens _ (TCbindP #a #b #wp #x #g pre post cg) sl0 res sl1;
+            <==> {_ by T.(apply_lemma (`U.iff_refl); trefl ())}
+              bind_pure_ens wp (fun x -> M.tree_ens (g x) (cg x)) sl0 res sl1;
+            <==> {
+              assert (M.tree_req _ (TCbindP #a #b #wp #x #g pre post cg) sl0
+                   == (wp (fun x -> M.tree_req (g x) (cg x) sl0) /\ True))
+                 by T.(trefl ());
+              U.prop_equal (fun p -> p) (M.tree_req _ (TCbindP #a #b #wp #x #g pre post cg) sl0)
+                                     (wp (fun x -> M.tree_req (g x) (cg x) sl0) /\ True);
+              FStar.Monotonic.Pure.elim_pure_wp_monotonicity wp;
+              introduce forall (x : a).
+                 as_ensures wp x ==>
+                 (M.tree_ens (g x) (cg x) sl0 res sl1 <==> tree_ens (repr_ST_of_M (g x) (cg x)) sl0 res sl1)
+               with introduce _ ==> _
+               with _ . repr_ST_of_M_ens (g x) (cg x) sl0 res sl1
+            }
+              as_requires wp /\ (exists (x : a) . as_ensures wp x /\ tree_ens (repr_ST_of_M (g x) (cg x)) sl0 res sl1);
+            <==> {_ by T.(apply_lemma (`U.iff_refl); trefl ())}
+              tree_ens (repr_ST_of_M _ (TCbindP #a #b #wp #x #g pre post cg)) sl0 res sl1;
+            <==> {U.f_equal tree_ens (repr_ST_of_M _ (TCbindP #a #b #wp #x #g pre post cg))
+                                   (repr_ST_of_M _ c)}
+              tree_ens (repr_ST_of_M _ c) sl0 res sl1;
+            }
+#pop-options
+
+
+
+(* --------------------------- *)
+
+open Steel.Reference
+
+let test_ST (r : ref nat) = repr_ST_of_M (test r).repr_tree (test_cond r)
+
+//let _ = fun r ->
+//  assert (print_util (test_ST r))
+//    by T.(norm normal_spec_steps; qed ())
